ReactorModel/Execution/Theorems/Variability/Basic.lean
@@ -24,30 +24,73 @@ def FiniteVariability (α) [Hierarchical α] : Prop :=
   ∀ g s, ∃ b, ∀ {s' : State α} (e : Execution s s'),
     (s'.tag < g) → e.length < b
 
+private def LoopModel.state₀ (microstep : Nat) : State LoopModel.Rtr where
+  rtr := { act := true }
+  tag := ⟨0, microstep⟩
+  progress := ∅
+  events
+    | .r => none
+    | .a => actionEvents microstep
+where
+  actionEvents : Nat → Time.Tag ⇉ Bool
+    | 0 => .singleton ⟨0, 0⟩ true
+    | n + 1 => sorry -- TODO: The execution semantics don't include deleting old events.
+
+private def LoopModel.execution₀ : (microstep : Nat) → Execution (state₀ 0) (state₀ microstep)
+  | 0     => .refl
+  | m + 1 =>
+    let e := execution₀ m
+    let s₁ := state₀ m
+    let s₂ := s₁.record .r
+    let s₃ := state₀ (m + 1)
+    have hs : { s₂ with tag := ⟨0, m + 1⟩ } = s₃ := sorry
+    let timeStep : s₂ ↓ₜ s₃ := hs ▸ sorry -- .Step.Time.mk sorry sorry sorry
+    .trans (.trans (execution₀ m) (.exec <| execStep m)) (.time timeStep)
+where
+  execStep (m) : (state₀ m) ↓ₑ (state₀ m |>.record .r) :=
+    .mk
+      {
+        mem := by
+          simp only [Partial.mem_iff, Hierarchical.obj?]
+          exists LoopModel.Rtr.rcn
+          split
+          case isTrue h =>
+            have o := h.choose_spec
+            obtain ⟨_, ho⟩ := h
+            rw [o.unique ho]
+            cases ho; cases ‹Member ..›; cases ‹StrictMember ..›
+            all_goals simp only [state₀, get?] at ‹_ = some _›
+            next _ h => injection h with h; subst h; rfl
+            next _ h => contradiction
+          case isFalse h =>
+            push_neg at h
+            exact h _ ⟨.strict (.final rfl)⟩ |>.elim
+        deps := by
+          intro i h
+          rw [dependencies, Set.mem_setOf] at h
+          -- h should be a contradiction, as r doesnt have any dependencies
+          sorry
+        unprocessed _ := by contradiction
+      }
+      (by sorry)
+      (by sorry)
+
+
+private theorem LoopModel.execution₀_length_le (microstep : Nat) :
+    microstep ≤ (execution₀ microstep).length := by
+  induction microstep
+  case zero => rfl
+  case succ => rw [execution₀, length, length]; omega
+
 -- Properness of a finite reactor model is not sufficient for finite variability. This is a
 -- consequence of logical tags being super-dense.
 --
 -- Proof Idea: Construct a reactor with a reaction which always schedules and action for the
 --             current logical time. This only ever increases the micro-step, but not the time.
+open LoopModel in
 theorem not_finitely_variable : ¬∀ (α) [Proper α] [Reactor.Finite α], FiniteVariability α := by
   intro h
-  let s₁ : State LoopModel.Rtr := {
-    rtr := { act := true },
-    tag := ⟨0, 0⟩,
-    progress := ∅,
-    events
-      | .r => none
-      | .a => some <| .singleton ⟨0, 0⟩ true
-  }
-  have ⟨b, h⟩ := h _ ⟨1, 0⟩ s₁
-  let s₂ : State LoopModel.Rtr := {
-    rtr := { act := true },
-    tag := ⟨0, b⟩,
-    progress := ∅,
-    events
-      | .r => none
-      | .a => sorry -- TODO: The execution semantics don't include deleting old events.
-  }
-  let e : Execution s₁ s₂ := sorry -- TODO: Construct this recursively.
-  have hl : e.length = b := sorry
-  exact lt_irrefl b (hl ▸ h e Time.Tag.lt_of_lt_time)
+  have ⟨b, h⟩ := h _ ⟨1, 0⟩ (state₀ 0)
+  have := h (execution₀ b) Time.Tag.lt_of_lt_time
+  have := execution₀_length_le b
+  omega
